\begin{array}{l}
\textbf{Formula:} (P \land (Q \lor R) \rightarrow (S \leftrightarrow T))\\ \textbf{Remove equivalences:} (P \land (Q \lor R) \rightarrow S \land T \lor  \neg S \land  \neg T)\\ \textbf{Remove implications:}  \neg (P \land (Q \lor R)) \lor S \land T \lor  \neg S \land  \neg T\\ \textbf{Push negations:} \neg P \lor \neg Q \land \neg R \lor S \land T \lor \neg S \land \neg T\\ \textbf{Distribute disjunctions:} (\neg P \lor \neg Q \lor S \lor \neg S) \land (\neg P \lor \neg Q \lor S \lor \neg T) \land (\neg P \lor \neg Q \lor T \lor \neg S) \land (\neg P \lor \neg Q \lor T \lor \neg T) \land (\neg P \lor \neg R \lor S \lor \neg S) \land (\neg P \lor \neg R \lor S \lor \neg T) \land (\neg P \lor \neg R \lor T \lor \neg S) \land (\neg P \lor \neg R \lor T \lor \neg T)\\
\end{array}